part A done

code/Map.dfy
@@ -19,14 +19,14 @@ module Map {
   type Entry<T> = (int, T)
 
   // Auxiliary function that can be used in contracts
-  function key<T>(e: Entry<T>): int
+  ghost function key<T>(e: Entry<T>): int
   {
     match e
     case (k, _) =>  k
   }
 
    // Auxiliary function that can be used in contracts
- function value<T>(e: Entry<T>): T
+  ghost function value<T>(e: Entry<T>): T
   {
     match e
     case (_, v) =>  v
@@ -38,24 +38,42 @@ module Map {
   ghost function entries<T(!new)>(m: Map<T>): set<Entry<T>>
   { L.elements(m) }
 
+  ghost function distinct<T(!new)>(m: Map<T>): bool
+  {
+    match m
+    case Nil => true
+    case Cons(x, tl) => x !in entries(tl) && distinct(tl)
+  }
+
+  ghost function distinctKeys<T(!new)>(m: Map<T>): bool
+  {
+    match m
+    case Nil => true
+    case Cons((k, v), tl) => (!exists e | e in entries(tl) :: key(e) == k) && distinctKeys(tl)
+  }
+
   // A map m is valid iff it contains no repeated elements and
   // every key in m has exactly one associated value (no contract needed) 
   ghost predicate isValid<T(!new)>(m: Map<T>)
   {
-    true // replace this line with your definition
+    distinct(m) && distinctKeys(m)
   }
 
   // For every value type T, emptyMap<T>() is 
   // the empty map of elements of type T
-  function emptyMap<T(!new)>(): Map<T> 
+  function emptyMap<T(!new)>(): Map<T>
+    ensures isValid<T>(emptyMap())
   { Nil }
 
   // isEmpty(m) is true iff m has no entries 
   predicate isEmpty<T>(m: Map<T>)
+    requires isValid(m)
   { m == Nil }
 
   // size(m) is the number of entries in m
   function size<T(==)>(m: Map<T>): nat 
+    requires isValid<T>(m)
+    ensures size<T>(m) == |entries<T>(m)|
   {
     match m
     case Nil => 0
@@ -64,6 +82,8 @@ module Map {
 
   // keys(m) is the set of keys in m's entries
   function keys<T(!new)>(m: Map<T>): set<int>
+    requires isValid(m)
+    ensures forall k :: k in keys(m) <==> exists v :: (k, v) in entries(m)
   {
     match m
     case Nil => {}
@@ -72,6 +92,8 @@ module Map {
 
   // values(m) is the set of values in m's entries
   function values<T(!new)>(m: Map<T>): set<T>
+    requires isValid(m)
+    ensures forall v :: v in values(m) <==> exists k :: (k, v) in entries(m)
   {
     match m
     case Nil => {}
@@ -82,6 +104,9 @@ module Map {
   // More precisely, it is Some(v) if k has an associated value v,
   // and is None otherwhise.
   function get<T(!new)>(m: Map<T>, k: int): Option<T>
+    requires isValid(m)
+    ensures k in keys(m) ==> exists v :: get(m, k) == Some(v) && (k, v) in entries(m)
+    ensures k !in keys(m) ==> get(m, k) == None
   {
     match m
     case Nil => None
@@ -95,6 +120,10 @@ module Map {
   // remove(m, k) is the map obtained from m by removing from it
   // the entry with key k, if any.
   function remove<T(!new)>(m: Map<T>, k: int): Map<T>
+    requires isValid(m)
+    ensures isValid(m)
+    ensures k in keys(m) ==> exists v :: (k, v) in entries(m) && entries(remove(m, k)) == entries(m) - {(k, v)}
+    ensures k !in keys(m) ==> entries(remove(m, k)) == entries(m)
   {
     match m
     case Nil => Nil
@@ -109,6 +138,10 @@ module Map {
   // put(m, k, v) is the map that associates key k with value v
   // and is othewise identical to m.
   function put<T(!new)>(m: Map<T>, k: int, v: T): Map<T>
+    requires isValid(m)
+    ensures isValid(put(m, k, v))
+    ensures k in keys(m) ==> exists v' :: (k, v') in entries(m) && entries(put(m, k, v)) == entries(m) - {(k, v')} + {(k, v)}
+    ensures k !in keys(m) ==> entries(put(m, k, v)) == entries(m) + {(k, v)}
   {
     match m
     case Nil => Cons((k, v), Nil)
